understanding refinement relations

theories/Compositional_Structures/Basic_Modules/Component_Types/Social_Choice_Types/RefinementList.thy
@@ -1,15 +1,32 @@
 theory RefinementList
   imports Verified_Voting_Rule_Construction.Preference_Relation
   Verified_Voting_Rule_Construction.Preference_List
+
+  Verified_Voting_Rule_Construction.Profile
+  Verified_Voting_Rule_Construction.Profile_List
+
   Refine_Imperative_HOL.IICF
 
 begin
 
 abbreviation "ballot_rel \<equiv> br (pl_\<alpha>) (well_formed_pl)"
 
-lemma aboveref: 
+lemma linearorder_ref: 
+  "(linear_order_on_l, linear_order_on) \<in> \<langle>Id\<rangle>set_rel \<rightarrow> ballot_rel \<rightarrow> bool_rel"                                 
+proof (refine_vcg, clarsimp_all)
+  fix alts:: "'a set"
+  fix bal:: "'a Preference_List" and bar:: "'a Preference_Relation"
+  assume "(bal, bar) \<in> ballot_rel"
+  from this show " linear_order_on_l alts bal = linear_order_on alts bar"
+  using in_br_conv linorder_l_imp_rel linorder_rel_imp_l
+    by metis
+qed
+  
+
+
+lemma aboveref:                                          
   shows "(above_l, above) \<in> ballot_rel \<rightarrow> Id \<rightarrow> \<langle>Id\<rangle>list_set_rel"
-  apply (refine_vcg)
+  apply (refine_vcg)                                    
   apply (auto simp add: refine_rel_defs)
   unfolding list_set_rel_def
   by (metis Id_O_R above_l_def aboveeq brI distinct_take list_rel_id_simp well_formed_pl_def)
@@ -24,18 +41,36 @@ lemma rankref:
 lemma is_less_preferred_than_ref:
   shows "(is_less_preferred_than_l, is_less_preferred_than) 
     \<in> Id \<rightarrow> ballot_rel \<rightarrow> Id \<rightarrow> bool_rel"
-  apply (refine_vcg rankeq)
+  apply (refine_vcg)
   by (auto simp only: refine_rel_defs less_preffered_l_rel_eq)
 
 lemma limitref:
   shows "(limit_l, limit) \<in> \<langle>Id\<rangle>set_rel \<rightarrow> ballot_rel \<rightarrow> ballot_rel"
-  apply (refine_vcg rankeq)
+  apply (refine_vcg)
   apply (auto simp add: refine_rel_defs)
-  unfolding well_formed_pl_def pl_\<alpha>_def
+  oops
+  (*unfolding well_formed_pl_def pl_\<alpha>_def
   apply auto
   apply (simp_all add: member_def)
-   apply clarsimp_all
-  oops
-   
+   apply clarsimp_all*)
+
+abbreviation "profile_rel \<equiv> \<langle>ballot_rel\<rangle>list_rel"
+
+lemma profileref:
+  shows "(profile_l, profile) \<in> \<langle>Id\<rangle>set_rel \<rightarrow> profile_rel \<rightarrow> bool_rel"
+  apply (refine_rcg linearorder_ref)
+ apply (clarsimp simp add: linearorder_ref)
+proof (-)
+  fix pl:: "'a Profile_List" 
+  fix pr:: "'a Profile"
+  assume prel: "(pl, pr) \<in> profile_rel"
+  fix A:: "'a set"
+  fix i:: nat
+  from prel have "\<forall>idx < length pl. ((pl!idx), (pr!idx)) \<in> ballot_rel"
+    using in_br_conv
+    by (simp add: list_rel_pres_length param_nth)
+  from prel this show " profile_l A pl =profile A pr" using in_br_conv  profile_def profile_l_def
+    by (metis linorder_l_imp_rel linorder_rel_imp_l list_rel_pres_length)
+qed
 
 end
